added more hash oracles

SQIR/OracleExample.v
@@ -152,6 +152,8 @@ Definition dr_qexp x0 x1 x2 x3 x4 x5 x6 x7 x8 x9 x10 x11 x12 x13 x14 x15 :=
   qr_qexp x2 x7 x8 x13;;;
   qr_qexp x3 x4 x9 x14.
 
+Definition dec2checker P `{Dec P} := checker (dec2bool P).
+
 Module DRTesting.
 
   Definition tmp : var := 16.
@@ -182,6 +184,63 @@ Module DRTesting.
 
   Definition dr_env : f_env := fun _ => 32.
 
+  Definition dr_oracle_spec : Checker :=
+    forAllShrink arbitrary shrink (fun v0 =>
+    forAllShrink arbitrary shrink (fun v1 =>
+    forAllShrink arbitrary shrink (fun v2 =>
+    forAllShrink arbitrary shrink (fun v3 =>
+    forAllShrink arbitrary shrink (fun v4 =>
+    forAllShrink arbitrary shrink (fun v5 =>
+    forAllShrink arbitrary shrink (fun v6 =>
+    forAllShrink arbitrary shrink (fun v7 =>
+    forAllShrink arbitrary shrink (fun v8 =>
+    forAllShrink arbitrary shrink (fun v9 =>
+    forAllShrink arbitrary shrink (fun v10 =>
+    forAllShrink arbitrary shrink (fun v11 =>
+    forAllShrink arbitrary shrink (fun v12 =>
+    forAllShrink arbitrary shrink (fun v13 =>
+    forAllShrink arbitrary shrink (fun v14 =>
+    forAllShrink arbitrary shrink (fun v15 =>
+    let
+      '(x0', x1', x2', x3', x4', x5', x6', x7',
+        x8', x9', x10', x11', x12', x13', x14', x15') :=
+      dr_spec
+        (bvector2bits v0) (bvector2bits v1) (bvector2bits v2) (bvector2bits v3)
+        (bvector2bits v4) (bvector2bits v5) (bvector2bits v6) (bvector2bits v7)
+        (bvector2bits v8) (bvector2bits v9)
+        (bvector2bits v10) (bvector2bits v11)
+        (bvector2bits v12) (bvector2bits v13)
+        (bvector2bits v14) (bvector2bits v15)
+    in
+    let v0' := bits2bvector x0' in
+    let v1' := bits2bvector x1' in
+    let v2' := bits2bvector x2' in
+    let v3' := bits2bvector x3' in
+    let v4' := bits2bvector x4' in
+    let v5' := bits2bvector x5' in
+    let v6' := bits2bvector x6' in
+    let v7' := bits2bvector x7' in
+    let v8' := bits2bvector x8' in
+    let v9' := bits2bvector x9' in
+    let v10' := bits2bvector x10' in
+    let v11' := bits2bvector x11' in
+    let v12' := bits2bvector x12' in
+    let v13' := bits2bvector x13' in
+    let v14' := bits2bvector x14' in
+    let v15' := bits2bvector x15' in
+    dec2checker
+    (st_equiv (get_vars dr_pexp) dr_env (get_prec dr_env dr_pexp)
+     (prog_sem dr_env dr_pexp
+        (0 |=> v0, 1 |=> v1, 2 |=> v2, 3 |=> v3,
+         4 |=> v4, 5 |=> v5, 6 |=> v6, 7 |=> v7,
+         8 |=> v8, 9 |=> v9, 10 |=> v10, 11 |=> v11,
+         12 |=> v12, 13 |=> v13, 14 |=> v14, 15 |=> v15))
+     (0 |=> v0', 1 |=> v1', 2 |=> v2', 3 |=> v3',
+      4 |=> v4', 5 |=> v5', 6 |=> v6', 7 |=> v7',
+      8 |=> v8', 9 |=> v9', 10 |=> v10', 11 |=> v11',
+      12 |=> v12', 13 |=> v13', 14 |=> v14', 15 |=> v15')))))))))))))))))).
+
+  (*
   Conjecture dr_oracle_spec :
     forall v0 v1 v2 v3 v4 v5 v6 v7 v8 v9 v10 v11 v12 v13 v14 v15,
     let
@@ -221,10 +280,207 @@ Module DRTesting.
    4 |=> v4', 5 |=> v5', 6 |=> v6', 7 |=> v7',
    8 |=> v8', 9 |=> v9', 10 |=> v10', 11 |=> v11',
    12 |=> v12', 13 |=> v13', 14 |=> v14', 15 |=> v15').
+   *)
 
 End DRTesting.
 
+(*
 QuickChickWith (updMaxSuccess stdArgs 1) DRTesting.dr_oracle_spec.
+ *)
+
+Fixpoint chacha_qexp' n x0 x1 x2 x3 x4 x5 x6 x7 x8 x9 x10 x11 x12 x13 x14 x15 :=
+  match n with
+  | 0 => skip
+  | S n' =>
+      dr_qexp x0 x1 x2 x3 x4 x5 x6 x7 x8 x9 x10 x11 x12 x13 x14 x15;;;
+      chacha_qexp' n' x0 x1 x2 x3 x4 x5 x6 x7 x8 x9 x10 x11 x12 x13 x14 x15
+  end.
+
+Definition chacha_qexp := chacha_qexp' 10.
+
+Fixpoint chacha_spec' n v0 v1 v2 v3 v4 v5 v6 v7 v8 v9 v10 v11 v12 v13 v14 v15 :=
+  match n with
+  | 0 => (v0, v1, v2, v3, v4, v5, v6, v7, v8, v9, v10, v11, v12, v13, v14, v15)
+  | S n' =>
+      let
+        '(v0', v1', v2', v3', v4', v5', v6', v7',
+          v8', v9', v10', v11', v12', v13', v14', v15') :=
+        dr_spec v0 v1 v2 v3 v4 v5 v6 v7 v8 v9 v10 v11 v12 v13 v14 v15
+      in
+      chacha_spec' n' v0' v1' v2' v3' v4' v5' v6' v7'
+                      v8' v9' v10' v11' v12' v13' v14' v15'
+  end.
+
+Definition chacha_spec := chacha_spec' 10.
+
+Module ChaChaTesting.
+
+  Definition tmp : var := 16.
+  Definition stack : var := 17.
+
+  Definition chacha_vmap : qvar * nat -> var :=
+    fun '(x, _) =>
+    match x with
+    | L x' => x'
+    | G x' => x'
+    end.
+
+  Definition chacha_benv := gen_genv (map (fun x => (Nat, x)) (seq 0 16)).
+
+  Definition compile_chacha :=
+    trans_qexp
+    0 32 (fun _ => 1) chacha_vmap chacha_benv (Reg.empty _) tmp stack 0 nil
+    (chacha_qexp (G 0) (G 1) (G 2) (G 3) (G 4) (G 5) (G 6) (G 7)
+             (G 8) (G 9) (G 10) (G 11) (G 12) (G 13) (G 14) (G 15)).
+
+  Definition chacha_pexp : pexp.
+  Proof.
+    destruct (compile_chacha) eqn:E1.
+    - destruct p, p, o.
+      + apply p.
+      + discriminate.
+    - discriminate.
+  Defined.
+
+  Definition chacha_env : f_env := fun _ => 32.
+
+  Definition chacha_oracle_spec : Checker :=
+    forAllShrink arbitrary shrink (fun v0 =>
+    forAllShrink arbitrary shrink (fun v1 =>
+    forAllShrink arbitrary shrink (fun v2 =>
+    forAllShrink arbitrary shrink (fun v3 =>
+    forAllShrink arbitrary shrink (fun v4 =>
+    forAllShrink arbitrary shrink (fun v5 =>
+    forAllShrink arbitrary shrink (fun v6 =>
+    forAllShrink arbitrary shrink (fun v7 =>
+    forAllShrink arbitrary shrink (fun v8 =>
+    forAllShrink arbitrary shrink (fun v9 =>
+    forAllShrink arbitrary shrink (fun v10 =>
+    forAllShrink arbitrary shrink (fun v11 =>
+    forAllShrink arbitrary shrink (fun v12 =>
+    forAllShrink arbitrary shrink (fun v13 =>
+    forAllShrink arbitrary shrink (fun v14 =>
+    forAllShrink arbitrary shrink (fun v15 =>
+    let
+      '(x0', x1', x2', x3', x4', x5', x6', x7',
+        x8', x9', x10', x11', x12', x13', x14', x15') :=
+      chacha_spec
+        (bvector2bits v0) (bvector2bits v1) (bvector2bits v2) (bvector2bits v3)
+        (bvector2bits v4) (bvector2bits v5) (bvector2bits v6) (bvector2bits v7)
+        (bvector2bits v8) (bvector2bits v9)
+        (bvector2bits v10) (bvector2bits v11)
+        (bvector2bits v12) (bvector2bits v13)
+        (bvector2bits v14) (bvector2bits v15)
+    in
+    let v0' := bits2bvector x0' in
+    let v1' := bits2bvector x1' in
+    let v2' := bits2bvector x2' in
+    let v3' := bits2bvector x3' in
+    let v4' := bits2bvector x4' in
+    let v5' := bits2bvector x5' in
+    let v6' := bits2bvector x6' in
+    let v7' := bits2bvector x7' in
+    let v8' := bits2bvector x8' in
+    let v9' := bits2bvector x9' in
+    let v10' := bits2bvector x10' in
+    let v11' := bits2bvector x11' in
+    let v12' := bits2bvector x12' in
+    let v13' := bits2bvector x13' in
+    let v14' := bits2bvector x14' in
+    let v15' := bits2bvector x15' in
+    dec2checker
+    (st_equiv
+     (get_vars chacha_pexp) chacha_env (get_prec chacha_env chacha_pexp)
+     (prog_sem chacha_env chacha_pexp
+        (0 |=> v0, 1 |=> v1, 2 |=> v2, 3 |=> v3,
+         4 |=> v4, 5 |=> v5, 6 |=> v6, 7 |=> v7,
+         8 |=> v8, 9 |=> v9, 10 |=> v10, 11 |=> v11,
+         12 |=> v12, 13 |=> v13, 14 |=> v14, 15 |=> v15))
+     (0 |=> v0', 1 |=> v1', 2 |=> v2', 3 |=> v3',
+      4 |=> v4', 5 |=> v5', 6 |=> v6', 7 |=> v7',
+      8 |=> v8', 9 |=> v9', 10 |=> v10', 11 |=> v11',
+      12 |=> v12', 13 |=> v13', 14 |=> v14', 15 |=> v15')))))))))))))))))).
+
+End ChaChaTesting.
+
+(*
+QuickChickWith (updMaxSuccess stdArgs 1) ChaChaTesting.chacha_oracle_spec.
+ *)
+
+Module Collision.
+
+Definition x0 : qvar := L 0.
+Definition x1 : qvar := L 1.
+Definition x2 : qvar := L 2.
+Definition x3 : qvar := L 3.
+Definition x4 : qvar := L 4.
+Definition x5 : qvar := L 5.
+Definition x6 : qvar := L 6.
+Definition x7 : qvar := L 7.
+Definition x8 : qvar := L 8.
+Definition x9 : qvar := L 9.
+Definition x10 : qvar := L 10.
+Definition x11 : qvar := L 11.
+Definition x12 : qvar := L 12.
+Definition x13 : qvar := L 13.
+Definition x14 : qvar := L 14.
+Definition x15 : qvar := L 15.
+Definition out : qvar := G 16.
+
+Definition collision_qexp
+  (v0 v1 v2 v3 v4 v5 v6 v7 v8 v9 v10 v11 v12 v13 v14 v15 : DWORD) :=
+  chacha_qexp x0 x1 x2 x3 x4 x5 x6 x7 x8 x9 x10 x11 x12 x13 x14 x15;;;
+  qif (ceq QFTA Nat (Nor (Var x0)) (Nor (Num (getBit v0))))
+  (qif (ceq QFTA Nat (Nor (Var x1)) (Nor (Num (getBit v1))))
+  (qif (ceq QFTA Nat (Nor (Var x2)) (Nor (Num (getBit v2))))
+  (qif (ceq QFTA Nat (Nor (Var x3)) (Nor (Num (getBit v3))))
+  (qif (ceq QFTA Nat (Nor (Var x4)) (Nor (Num (getBit v4))))
+  (qif (ceq QFTA Nat (Nor (Var x5)) (Nor (Num (getBit v5))))
+  (qif (ceq QFTA Nat (Nor (Var x6)) (Nor (Num (getBit v6))))
+  (qif (ceq QFTA Nat (Nor (Var x7)) (Nor (Num (getBit v7))))
+  (qif (ceq QFTA Nat (Nor (Var x8)) (Nor (Num (getBit v8))))
+  (qif (ceq QFTA Nat (Nor (Var x9)) (Nor (Num (getBit v9))))
+  (qif (ceq QFTA Nat (Nor (Var x10)) (Nor (Num (getBit v10))))
+  (qif (ceq QFTA Nat (Nor (Var x11)) (Nor (Num (getBit v11))))
+  (qif (ceq QFTA Nat (Nor (Var x12)) (Nor (Num (getBit v12))))
+  (qif (ceq QFTA Nat (Nor (Var x13)) (Nor (Num (getBit v13))))
+  (qif (ceq QFTA Nat (Nor (Var x14)) (Nor (Num (getBit v14))))
+  (qif (ceq QFTA Nat (Nor (Var x15)) (Nor (Num (getBit v15))))
+  (init Bl (Nor (Var out)) (Nor (Num (fun _ => true))))
+  skip) skip) skip) skip) skip) skip) skip) skip)
+  skip) skip) skip) skip) skip) skip) skip) skip.
+
+(*
+Definition collision_spec
+  (v0 v1 v2 v3 v4 v5 v6 v7 v8 v9 v10 v11 v12 v13 v14 v15 
+  v0' v1' v2' v3' v4' v5' v6' v7' v8' v9' v10' v11' v12' v13' v14' v15' : DWORD)
+  :=
+  let
+    '(v0'', v1'', v2'', v3'', v4'', v5'', v6'', v7'',
+    v8'', v9'', v10'', v11'', v12'', v13'', v14'', v15'') :=
+    chacha_spec v0 v1 v2 v3 v4 v5 v6 v7 v8 v9 v10 v11 v12 v13 v14 v15
+  in
+  eqtype.eq_op v0' v0'' &&
+  eqtype.eq_op v1' v1'' &&
+  eqtype.eq_op v2' v2'' &&
+  eqtype.eq_op v3' v3'' &&
+  eqtype.eq_op v4' v4'' &&
+  eqtype.eq_op v5' v5'' &&
+  eqtype.eq_op v6' v6'' &&
+  eqtype.eq_op v7' v7'' &&
+  eqtype.eq_op v8' v8'' &&
+  eqtype.eq_op v9' v9'' &&
+  eqtype.eq_op v10' v10'' &&
+  eqtype.eq_op v11' v11'' &&
+  eqtype.eq_op v12' v12'' &&
+  eqtype.eq_op v13' v13'' &&
+  eqtype.eq_op v14' v14'' &&
+  eqtype.eq_op v15' v15''.
+ *)
+
+End Collision.
+
+Open Scope list_scope.
 
 Definition g :var := 1.
 Definition x :var := 7.
@@ -235,22 +491,8 @@ Definition d :var := 100.
 Definition f :var := 8.
 Definition result :var := 9.
 
-Definition hash_oracle (key:nat) (sndk:nat) :=
-     (f, ((Bl,g,1)::(Nat,x,1)::(Nat,a,1)::(Nat,b,1)::(Nat,c,1)::(Nat,d,1)::[]),
-      init Nat (Nor (Var (L d))) (Nor (Num (nat2fb 1)));;;
-      qfor x (Nor (Num (nat2fb 10)))
-           (hash_qr (L a) (L c);;; hash_qr (L b) (L d) ;;; hash_qr (L a) (L d)
-                ;;; hash_qr (L b) (L c);;; nadd Classic (Nor (Num (nat2fb 1))) (Nor (Var (L x))));;;
-      qif (ceq QFTA Nat (Nor (Var (L c))) (Nor (Num (nat2fb key))))
-                (qif (ceq QFTA Nat (Nor (Var (L d))) (Nor (Num (nat2fb sndk))))
-                    (init Bl (Nor (Var (L g))) (Nor (Num (nat2fb 1)))) (skip)) (skip), L g).
-
-Definition hash_prog (s_size:nat) (size:nat) (key:nat) (sndk:nat) : prog := 
-         (s_size, size,[(Bl,result)],[hash_oracle key sndk],f,result).
-
 (* define sin/cos. a = x^2, b = x^1/3/5/...., d is the result
     the input of sin/cos function is x/2 (not x) range from [0,pi/2) *)
-
 
 Definition x2 := 6.
 Definition x3 := 0.
